Done!

fullImpliesPartial.v
@@ -1,184 +1,223 @@
-Require Export partialImpliesFull.  
-
+Require Export AheadOfNI.  
+Require Export partialImpliesFull.
 
 (*
  * If we can replay from one state to another and the first state is
  * invalid, then the second one must be too
  *)
-Theorem replayInvalid : forall b1 b2 H H' rv wv tid e0 L e L' e' chkpnt HI, 
-                          replay H (txThread b1 tid rv e0 L e) H' (txThread b2 tid rv e0 L' e') ->
+
+
+Theorem logMonotonic : forall H H' b tid rv e0 L e L' e',
+    replay H (txThread true tid rv e0 L e) H' (txThread b tid rv e0 L' e') ->
+    b = true. 
+Proof.
+  intros. dependent induction H0; auto.
+  {dependent destruction H0; eauto. }
+Qed. 
+ 
+Theorem replayInvalid : forall H H' rv wv tid e0 L e L' e' chkpnt HI, 
+                          replay H (txThread false tid rv e0 L e) H' (txThread false tid rv e0 L' e') ->
                           validate tid rv wv e0 L H (abort chkpnt HI) ->
                           validate tid rv wv e0 L' H (abort chkpnt HI).
 Proof.
-  intros. genDeps{{chkpnt; HI}}. dependent induction H0; intros; auto.
-  dependent destruction H0; eauto. 
-  {eapply IHreplay; eauto. eapply readPropAbort; eauto.
-   constructor. }
-  {eapply IHreplay; eauto. eapply readPropAbort; eauto.
-   constructor. }
-  {eapply IHreplay; eauto. eapply readPropAbort; eauto.
-   dependent destruction H4; constructor. }
-Admitted. 
-
-(*
-
-(*if the beginning of a replay aborts, then so does the endpoint*)
-Theorem abortReplay : forall S L H C L' e' e'' L'' e e0, 
-                        replay H (Some(S,e0),L,e) (Some(S,e0),L',e') ->
-                        validate S L H C (abort e'' L'') -> 
-                        validate S L' H C (abort e'' L''). 
-Proof.
   intros. dependent induction H0; auto.
-  inv H0; eapply IHreplay; eauto; eapply validateAbortPropogate; eauto. 
+  dependent destruction H0; eauto. 
+  {eapply IHreplay. eauto. eauto. eapply readPropAbort.
+   eauto. constructor. }
+  {eapply IHreplay. eauto. eauto. eapply readPropAbort.
+   eauto. dependent destruction H4. constructor. }
+  {eapply logMonotonic in H3. solveByInv. }
 Qed. 
- *)
-
-Inductive AheadOf (H : heap) : pool -> pool -> Prop :=
-| aheadOfNoTX : forall tid e, AheadOf H (Single(noTXThread tid e)) (Single(noTXThread tid e))
-| aheadOfTXRO : forall tid rv e0 L L' e e',
-    replay H (txThread false tid rv e0 L e) H (txThread false tid rv e0 L' e') ->
-    AheadOf H (Single(txThread false tid rv e0 L e)) (Single(txThread false tid rv e0 L' e'))
-| aheadOfTXRW : forall tid rv b e0 L e,
-    AheadOf H (Single(txThread b tid rv e0 L e)) (Single(txThread b tid rv e0 L e))
-| replayPar : forall T1 T2 T1' T2',
-    AheadOf H T1 T1' -> AheadOf H T2 T2' ->
-    AheadOf H (Par T1 T2) (Par T1' T2'). 
 
 Ltac sameStep :=
   match goal with
   |H : decompose ?t ?E ?e, H' : decompose ?t ?E' ?e' |- _ =>
    eapply decomposeDeterministic in H; eauto; invertHyp; repeat invertEq
-  end. 
+  end.
 
-Theorem logMonotonic : forall H H' tid rv e0 L e L' e',
-    replay H (txThread true tid rv e0 L e) H' (txThread false tid rv e0 L' e') -> False.
+Theorem AheadOfExtend : forall tid rv e0 L e''' L''' e H L' e' C,
+    rewind H (txThread false tid rv e0 L e) H (txThread false tid rv e0 L' e') ->
+    validate tid rv C e0 L H (commit (e''', L''') H H) -> C > rv ->
+    exists e'' L'', 
+    (validate tid rv C e0 L' H (commit (e'', L'') H H) /\
+     rewind H (txThread false tid rv e0 L e) H (txThread false tid rv e0 L' e')) \/
+    (validate tid rv C e0 L' H (abort (e'', L'') H) /\
+     rewind H (txThread false tid C e0 L e) H (txThread false tid C e0 L'' e'')).
 Proof.
-  intros. dependent induction H0.
-  {dependent destruction H0; eauto. }
+  intros. genDeps{{e'''; L'''}}. 
+  dependent induction H0; intros. 
+  {econstructor. econstructor. left. split. eauto. constructor. }
+  {dependent destruction H1. 
+   {eapply IHrewind in H4; auto. invertHyp. inv H4; invertHyp.
+    {econstructor. econstructor. left. split. econstructor; eauto.
+     econstructor. eauto. econstructor; eauto. }
+    {econstructor. econstructor. right. split. eapply readPropAbort; eauto.
+     constructor. assumption. } eauto. 
+   }
+   {dependent destruction H5. copy H6. eapply IHrewind in H6; auto. invertHyp.
+    inv H6; invertHyp.
+    {econstructor. econstructor. right. split. econstructor; eauto.
+     eapply rewindNewerStamp. eapply decomposeEq in H1. subst. eassumption.
+     omega. eauto. }
+    {econstructor. econstructor. right. split. eapply readPropAbort; eauto.
+     constructor. assumption. } eauto. 
+   }
+   {eapply IHrewind in H2; auto. invertHyp. inv H2; invertHyp.
+    {econstructor. econstructor. left. split; eauto. econstructor; eauto.
+     eapply r_atomicIdemStep; eauto. }
+    {econstructor. econstructor. right. split; eauto. } eauto. 
+   }
+   {eapply IHrewind in H2; auto. invertHyp. inv H2; invertHyp.
+    {econstructor. econstructor. left. split; eauto. econstructor; eauto.
+     eapply r_betaStep; eauto. }
+    {econstructor. econstructor. right. split; eauto. } eauto. 
+   }
+  }
 Qed. 
 
-
-Theorem AheadOfNI : forall C C' H H' T1 T1' T2 T2',
-    f_step C H T1 C' H' T1' -> AheadOf H T2 T2' ->
-    AheadOf H' T2 T2'.
-Proof.
-  intros. genDeps{{C; T1; C'; T1'}}. 
-  induction H1; intros.
-  {constructor. }
-  {dependent destruction H1.
-   {
-Admitted. 
-    
-                        
 (*partial abort can simulate full abort*)
 Theorem fullImpliesPartial : forall C H T C' H' T' PT, 
-                               f_step C H T C' H' T' -> AheadOf H T PT ->
-                               poolRewind C H PT -> poolRewind C H T ->
-                               exists PT', p_multistep C H PT C' H' PT' /\
-                                           AheadOf H' T' PT'.
+    f_step C H T C' H' T' -> AheadOf C H T PT ->
+    poolRewind C H PT -> poolRewind C H T ->
+    exists PT', p_multistep C H PT C' H' PT' /\
+           AheadOf C' H' T' PT'.
 Proof.
   intros. generalize dependent PT. induction H0; intros. 
   {(*lifted step (full abort)*)
     inv H0. dependent destruction H3. dependent destruction H4. 
-    {copy H0. eapply validateRewindHeapEq in H6; eauto. simpl in *.
+    {copy H0. eapply validateRewindHeapEq in H8; eauto. simpl in *.
      subst. eapply replayInvalid in H5; eauto.    
      assert(rewind H'0 (txThread false tid S e0 NilLog e0) H (txThread false tid S e0 L'0 e'0)).
-     rewrite <- rewindIFFReplay in H4. eapply rewindTrans; eassumption.
-     eapply abortRewind in H6; eauto; try omega. copy H5. 
+     rewrite <- rewindIFFReplay in H7. eapply rewindTrans; eassumption.
+     eapply abortRewind in H8; eauto; try omega. copy H5. 
      eapply validateValidate in H5. invertHyp. econstructor. split.
      eapply c_multi_step. eapply c_liftedStep. econstructor. eauto. 
-     constructor. econstructor. rewrite <- rewindIFFReplay. assumption. }
-    {copy H0. eapply validateRewindHeapEq in H4; eauto. simpl in *. subst. 
+     constructor. econstructor; eauto. rewrite <- rewindIFFReplay. assumption. }
+    {copy H0. eapply validateRewindHeapEq in H0; eauto. simpl in *. subst. 
      econstructor. split. eapply c_multi_step. eapply c_liftedStep.
-     econstructor; eauto. constructor. econstructor.
-     eapply abortRewind in H5; eauto; try omega. rewrite <- rewindIFFReplay. 
-     assumption. }
+     econstructor; eauto. constructor. econstructor; auto. 
+     eapply abortRewind in H5; eauto. rewrite <- rewindIFFReplay. auto. 
+     omega. }
   }
   {(*transactional step*)
     dependent destruction H0.
     {(*checkpoint read*)
       dependent destruction H3. dependent destruction H6.
-      {dependent destruction H6.
+      {dependent destruction H8.
        {econstructor. split. eapply c_multi_step.
         eapply c_transStep. econstructor; eauto. constructor.
-        econstructor. constructor. }
-       {dependent destruction H7; sameStep. 
+        econstructor; auto. constructor. }
+       {dependent destruction H9; sameStep. 
         {transEq. invertEq. econstructor. split. constructor.
-         econstructor. eauto. }
+         econstructor; eauto. }
         {transEq. invertEq. exfalso. eapply validInvalidStamp; eauto. }
        }
       }
       {econstructor. split. eapply c_multi_step.
         eapply c_transStep. econstructor; eauto. constructor.
-        econstructor. constructor. }
+        econstructor; eauto. constructor. }
     }
     {(*non-checkpoint read*)
       dependent destruction H3. dependent destruction H6.
       {econstructor. split. eapply c_multi_step.
        eapply c_transStep. econstructor; eauto. constructor.
-       econstructor. }
+       econstructor; auto. }
     }
     {(*write*)
       dependent destruction H3. dependent destruction H6.
-      {dependent destruction H6.
+      {dependent destruction H8.
        {econstructor. split. eapply c_multi_step.
         eapply c_transStep. eapply t_writeLocked; eauto.
-        constructor. econstructor. }
-       {dependent destruction H7; sameStep. exfalso.
-        eapply logMonotonic; eauto. }
+        constructor. econstructor; auto. }
+       {dependent destruction H9; sameStep. exfalso.
+        eapply logMonotonic in H11. solveByInv. }
       }
       {econstructor. split. eapply c_multi_step.
-        eapply c_transStep. eapply t_writeLocked; eauto.
-        constructor. econstructor. }
+       eapply c_transStep. eapply t_writeLocked; eauto.
+       constructor. econstructor; auto. }
     }
-    {dependent destruction H1. dependent destruction H2.
-     dependent destruction H1.
+    {dependent destruction H3. dependent destruction H4.
+     dependent destruction H6.
      {econstructor. split. eapply c_multi_step.
       eapply c_transStep. eapply t_atomicIdemStep; eauto.
-      constructor. econstructor. constructor. }
-     {dependent destruction H1; sameStep. econstructor.
-      split. constructor. econstructor. eauto. }
+      constructor. econstructor; auto. constructor. }
+     {dependent destruction H6; sameStep. econstructor.
+      split. constructor. econstructor; eauto. }
      {econstructor. split. eapply c_multi_step.
       eapply c_transStep. eapply t_atomicIdemStep; eauto.
-      constructor. econstructor. }
+      constructor. econstructor; auto. }
     }
-    {dependent destruction H1. dependent destruction H2.
-     dependent destruction H1.
+    {dependent destruction H3. dependent destruction H4.
+     dependent destruction H6.
      {econstructor. split. eapply c_multi_step.
       eapply c_transStep. eapply t_betaStep; eauto.
-      constructor. econstructor. constructor. }
-     {dependent destruction H1; sameStep. econstructor.
-      split. constructor. econstructor. eauto. }
+      constructor. econstructor; auto. constructor. }
+     {dependent destruction H6; sameStep. econstructor.
+      split. constructor. econstructor; eauto. }
      {econstructor. split. eapply c_multi_step.
       eapply c_transStep. eapply t_betaStep; eauto.
-      constructor. econstructor. }
+      constructor. econstructor; auto. }
     }
   }
-  {inv H1. dependent destruction H2. inv H3. eapply IHc_step in H6; eauto.
+  {inv H1. dependent destruction H2. inv H3. eapply IHc_step in H7; eauto.
    invertHyp. econstructor. split. eapply multi_L. eauto.
-   econstructor; eauto.
-
-   eapply AheadOfNI; eauto. }
-  {inv H1. inv H2. inv H3. eapply IHc_step in H8; eauto.
+   econstructor; eauto. Focus 2. eapply AheadOfNI; eauto.
+   eapply f_stepDisjoint. Focus 3. eassumption. auto. auto.
+   auto. }
+  {inv H1. inv H2. inv H3. eapply IHc_step in H9; eauto.
    invertHyp. econstructor. split. eapply multi_R. eauto.
-   econstructor; eauto. eapply AheadOfNI; eauto. }
+   econstructor; eauto. Focus 2. eapply AheadOfNI; eauto.
+   rewrite DisjointComm. auto. rewrite DisjointComm.
+   eapply f_stepDisjoint. Focus 3. eauto. auto. auto.
+   rewrite DisjointComm. auto. }
   {inv H1. inv H2. econstructor. split. eapply c_multi_step.
-   eapply c_forkStep; eauto. constructor. repeat constructor. }
+   eapply c_forkStep; eauto. constructor. repeat constructor; eauto.
+   intros. intro. simpl in *. solveIn. omega. }
   {inv H2. inv H3. econstructor. split. eapply c_multi_step.
-   eapply c_allocStep; eauto. constructor. constructor. }
-  {dependent destruction H2. dependent destruction H3.
-   dependent destruction H6. dependent destruction H5.
-   {econstructor. split. eapply c_multi_step. eapply c_commitStep; eauto.
-    constructor. constructor. }
-   {dependent destruction H5; sameStep. }
+   eapply c_allocStep; eauto. constructor. constructor. auto. }
+  {dependent destruction H3. dependent destruction H5.
+   {dependent destruction H8. dependent destruction H7.
+    {econstructor. split. eapply c_multi_step. eapply c_commitStep; eauto. 
+     constructor. econstructor. omega. }
+    {dependent destruction H7; sameStep. }
+   }
+   {dependent destruction H7. econstructor. split.
+    eapply c_multi_step. eapply c_commitStep; eauto. constructor.
+    econstructor. omega. }
   }
   {inv H1. inv H2. econstructor. split. eapply c_multi_step.
-   eapply c_atomicStep; eauto. constructor. econstructor. 
-   econstructor. }
+   eapply c_atomicStep; eauto. constructor. econstructor; eauto.
+   constructor. }
   {inv H1. inv H2. econstructor. split. eapply c_multi_step.
-   eapply c_betaStep; eauto. constructor. constructor. }
-  {admit. }
-Admitted. 
+   eapply c_betaStep; eauto. constructor. constructor; auto. }
+  {dependent destruction H3. dependent destruction H4.
+   {dependent destruction H7. copy H1. eapply rewindNoWrites in H1; eauto.
+    subst. copy H7. eapply rewindNoWrites in H7; eauto. subst.
+    copy H0. eapply validateNoWrites in H0; eauto. invertHyp. subst.
+    destruct chkpnt. eapply AheadOfExtend in H7; eauto. Focus 2.
+    rewrite rewindIFFReplay. eassumption. invertHyp. inv H0; invertHyp.
+    {econstructor. split. eapply c_multi_step. eapply c_tsExtend. eauto.
+     constructor. econstructor; auto. rewrite <- rewindIFFReplay.
+     eapply rewindNewerStamp; eauto. omega. }
+    {econstructor. split. eapply c_multi_step. eapply c_liftedStep.
+     econstructor. eauto. constructor. econstructor; eauto.
+     rewrite <- rewindIFFReplay. assumption. }
+   }
+   {econstructor. split. eapply c_multi_step. eapply c_tsExtend.
+    eauto. constructor. econstructor; auto. }
+  }
+Qed. 
+
+
+
+
+
+    
+
+           
+
+     
+     
 
 (*generalize step preserves rewind to thread pools*)
 Theorem multistepPreservesRewind : forall C H T C' H' T',
@@ -191,19 +230,18 @@ Qed.
 
 (*generalize full implies partial to thread pools*)
 Theorem fullImpliesPartialMulti : forall C H T C' H' T' PT, 
-                               f_multistep C H T C' H' T' -> AheadOf H T PT ->
-                               poolRewind C H PT ->
+                               f_multistep C H T C' H' T' -> AheadOf C H T PT ->
+                               poolRewind C H PT -> poolRewind C H T ->
                                exists PT', p_multistep C H PT C' H' PT' /\
-                                           AheadOf H' T' PT'.
+                                           AheadOf C' H' T' PT'.
 Proof.
   intros. generalize dependent PT. induction H0; intros. 
   {exists PT. split. constructor. auto. }
   {copy H0. eapply fullImpliesPartial in H0; eauto. invertHyp. 
-   copy H0. apply multistepPreservesRewind in H5; auto. 
-   eapply IHmultistep in H6; eauto. invertHyp. exists x0. split. 
-   eapply multi_trans; eauto. auto. }
+   copy H0. apply multistepPreservesRewind in H0; auto. 
+   eapply IHmultistep in H0; eauto. invertHyp. exists x0. split. 
+   eapply multi_trans; eauto. auto. eapply f_stepRewind; eauto. }
 Qed. 
-
 
 
 
